*rename exp to pow

SquareAndMultiply.dfy
@@ -1,10 +1,10 @@
-function exp(x: int, n: int): int
+function pow(x: int, n: int): int
     requires n >= 0
 {
     if n == 0 then 
         1
     else 
-        x * exp(x, n-1)
+        x * pow(x, n-1)
 }
 
 function isEven(a: int): bool
@@ -13,14 +13,18 @@ function isEven(a: int): bool
     a % 2 == 0
 }
 
+
+type EvenInt = x: nat | isEven(x) witness 2
+type OddInt = x: nat | !isEven(x) witness 3
+
 method NormalExp(x: int, n: int) returns (r: int)
 requires n > 0
-ensures r == exp(x, n)
+ensures r == pow(x, n)
 {
     r := x;
     var tmp := n - 1;
     while(tmp > 0)
-        invariant r == exp(x, n - tmp)
+        invariant r == pow(x, n - tmp)
     {
         r := r * x;
         tmp := tmp - 1;
@@ -30,11 +34,11 @@ ensures r == exp(x, n)
 lemma AssociativityLaw(x: int, n: int, m: int)
   requires n > 0
   requires m >= 0
-  ensures exp(x, n + m) == exp(x, n) * exp(x, m)
+  ensures pow(x, n + m) == pow(x, n) * pow(x, m)
 {	
     if (m == 0)
     {
-        assert(exp(x, n + 0) == exp(x,n));
+        assert(pow(x, n + 0) == pow(x,n));
     }
     else
     {
@@ -45,15 +49,15 @@ lemma AssociativityLaw(x: int, n: int, m: int)
 lemma AssociativityLaw2(x: int, n: int, m: int)
   requires n > 0
   requires m >= 0
-  ensures exp(x, n * m) == exp(exp(x, n), m)
+  ensures pow(x, n * m) == pow(pow(x, n), m)
 {
     if (m == 0)
     {
-        assert(exp(x, 0) == 1);
+        assert(pow(x, 0) == 1);
     }
     else
     {
-        assert(exp(x, n * m) == exp(x, n * (m-1) + n));		
+        assert(pow(x, n * m) == pow(x, n * (m-1) + n));		
         AssociativityLaw(x, n, (m-1) * n); // exp(x, m*n) = exp(x, n * (m-1)) * exp(x, n)		
         AssociativityLaw2(x, n, m - 1);	 // exp(x, n * (m-1)) = exp(exp(x, n), m - 1) 
     }
@@ -61,21 +65,21 @@ lemma AssociativityLaw2(x: int, n: int, m: int)
 
 method FastExpr(x2: int, n2: int) returns (r: int)
 requires n2 > 0
-ensures r == exp(x2, n2)
+ensures r == pow(x2, n2)
 {
     var x := x2;
     var n := n2;
     var y := 1;		
-    assert(y * exp(x, n) == exp(x2, n2));
+    assert(y * pow(x, n) == pow(x2, n2));
     while (n > 1)
         decreases n
         invariant n > 0
-        invariant y * exp(x, n) == exp(x2, n2) 	
+        invariant y * pow(x, n) == pow(x2, n2) 	
     {			
       if (!isEven(n))
       {
         AssociativityLaw2(x, 2, (n-1)/2);  // exp(x,n-1) == exp(exp(x, 2), (n-1)/2)     
-        y, x, n := x * y, exp(x, 2), (n-1)/2;	
+        y, x, n := x * y, pow(x, 2), (n-1)/2;	
         // y * exp(x , n) == y' * exp(x', (n - 1)/2)    
         // y' = x * y
         // x' = x * x
@@ -84,7 +88,7 @@ ensures r == exp(x2, n2)
       else
       {    
         AssociativityLaw2(x, 2, n / 2); // exp(x, n) == exp(exp(x, 2), n/2)		
-        y, x, n := y, exp(x, 2), n / 2; 
+        y, x, n := y, pow(x, 2), n / 2; 
         // y * exp(x , n) -> y' * exp(x', n/2)           
         // y' = y
         // x' = x * x  
